lemma chap1: manual; progress (WIP)

exercise-files/chap1.ec
@@ -19,14 +19,14 @@ module Func1 = {
      return type of procedures in the definition.
   *)
 
-  proc add_2 (x: int) : int = {return x+2; }
+  proc add_2 (x: int) : int = {x<- x + 2; return x; }
 }.
 
 (*
 EC allows us to define concretely defined procedures like we did above.
 But since we want to model adversaries about whom we know nothing,
 we can also define abstract procedures like an eavesdrop procedure 
-of an evil adversary. We don't what the procedure does, but we
+of an evil adversary. We don't know what the procedure does, but we
 do know its return type. We will return to this later when we
 start working with cryptographic protocols. But this is
 an important fact that we need to keep in mind.
@@ -45,38 +45,91 @@ module type Evil_adv = {
 (* 
 Let us return to hoare triples and take a look at some triples and
 try to prove them in EC.
-To declare a hoare triple we use the following syntax
+A triple denoted by {P} C {Q} in theory is expressed as
+hoare [C : P ==> Q ] in EC, with the usual definitions.
+Additionally, the return value of the program C, is stored in a special 
+keyword called res.
 *)
 
-lemma triple1: hoare [ Func1.add_1 : x = 1 ==> res = 2 ].
+lemma triple1: hoare [ Func1.add_1 : x = 1 ==> res = 2].
+proof.
+(*
+When working with hoare logic, or pHL, or pRHL, the goal will be different from
+what a goal in ambient logic looks like. We need to start stepping through
+the procedure or program that is being reasoned about and change the
+preconditions and postconditions according axioms and lemmas that we have.
+To make progress here, we first need to tell EC what Func1.add_1 is.
+The way to do that is by using the "proc" tactic.
+It simply fills in the definitions of the procedures that we define.
+*)
+proc.
+
+(*
+When the goal’s conclusion is a statement judgement whose program is empty,
+like we have now the "skip" tactic reduces it to the goal whose conclusion
+is the ambient logic formula P => Q,
+where P is the original conclusion’s precondition, 
+and Q is its postcondition.
+*)
+
+skip.
+
+(*
+Now we are back in familiar territory, except the fact that
+we have an interesting "&hr" lurking in the goal.
+This refers to the memory in which the program acts.
+When we deal with multiple programs, there is a possibility
+that the variables come from different memories. So EC provides us
+a different name spaces to deal with them.
+To introduce memory into the context we need to prepend "&" to a variable name.
+Like so:
+*)
+
+move => &m x.
+subst.
+(* The "subst" tactic simply substitutes variables *)
+trivial.
+qed.
+
+
+lemma triple2: hoare [ Func1.add_2 : x = 1 ==> res = 3 ].
 proof.
 proc.
 (*
-The proc tactic simply fills in the procedures with the
-definitions for both abstract and concrete procudures.
-*)
 
-(* TODO: Write about skip  *)
+Now we have a program which is not empty,
+so we can't use the skip tactic directly. 
+Thankfully we learnt about postcondition weakening.
+Take a look at this proof-tree. Applying the "wp" tactic
+computes the weakest precondition that needs to hold by
+consuming program statements and replacing the conclusion's
+postcondition with the weakest precondition R such that the 
+statement judgement consisting of R, the consumed suffix(es) and
+the conclusion’s original postcondition holds.
+
+                   x = 1  => x+2=3
+          -------------------------------skip
+                 {x = 1}     {x+2=3}
+          -------------------------------wp
+                {x = 1} x:= x+2 {x=3}
+
+  (* TODO: Show it formally once (Need help) *)
+*)
+wp.
 skip.
 move => &m x.
-(* TODO: Write about memory and subst *)
 subst.
 trivial.
 qed.
 
-lemma triple2: hoare [ Func1.add_1 : x = 1 ==> res = 3 ].
-proof.
-proc.
-skip.
-move => &m x.
-subst.
-(* 
-Clearly this isn't true.
-So to abort a proof, we simply use abort *)
-abort.
-
 (* Using some automation *)
 
+(*
+We generally don't want to be dealing with the low-level proofs,
+so we will be combining Hoare logic with the automated tactics that
+we saw previously. One thing to remember is that the automated tactics
+work well with ambient logic.
+*)
 module Func2 = {
   proc x_sq (x:int) : int = { return x*x; }
   proc x_0  (x:int) : int = { x <- x*x; x<- x-x; return x; }
@@ -87,27 +140,67 @@ lemma triple3: hoare [ Func2.x_sq : 4 <= x ==> 16 <= res ].
 proof.
 proc.
 skip.
+(*
+Here this conclusion is trivial for us to understand and prove on paper
+however it can be quite hard to do with EC, so we will simply outsource it to smt.
+The external provers are quite powerful, and can make our life easier.
+*)
 smt.
 qed.
 
+(*
+Now let us look at the special cases that we had in the text.
+Namely: {true} C {Q}, and {false} C {Q}.
+*)
 lemma triple4: hoare [ Func2.x_0 : true ==> res=0 ].
 proof.
 proc.
 wp.
 skip.
+move => &m t x.
 by simplify.
+(* Prepending the "by" keyword to a tactic
+tries to close the goals by applying trivial
+to the result of the tactic, and fails if the goal can't be closed *)
 qed.
 
+(*
+So far so good, that was pretty much what we expected.
+However let us take a look at the next lemma. Now we are looking at the triple:
+{false} x:=15 {x = 0}.
+This shouldn't hold, but watch what happens.
+*)
 
 lemma triple5: hoare [ Func2.f_15 : false ==> res=0 ].
 proof.
 proc.
 wp.
 skip.
-auto.
+move => _ f.
+(*
+The underscore essentially is a pattern for introduction 
+which tells EC to ignore whatever is in that position.
+Here since we have a "forall _" in the goal already, we tell EC to ignore it.
+You could also use a "?", to let EC decide what to call the variable being moved
+to the assumptions.
+*)
+
+(*
+Pause here for a moment and ponder about what the goal currently says.
+It says that assuming that "false" holds, we want to prove that 15 = 0.
+As absurd as it is, we know that "false" is the strongest statement there is.
+And we have arrived to a state we say that "false" holds. This would imply that anything and
+everything can be derived from false. Hence we can actually "prove" that 15 = 0.
+*)
+trivial.
 qed.
 
-(* Note about how this triple holds. Absurdity! *)
+(*
+The point to understand here is that we could only do this 
+because we moved "false" into the context manually when we used
+the "move" tactic. So our math is still consistent and the world hasn't exploded yet.
+The way to think about this triple is assuming "false" holds implies that 15 = 0.
+*)
 
 module Func3 = {
 
@@ -129,7 +222,7 @@ proof.
 proc.
 simplify.
 (* TODO: HELP! *)
-while (  i <= a /\ r = r * x  ).
+while ( r = r * x  ).
 wp.
 skip.
 auto.
